theories/LambdaWt/WtInContext.v
@@ -1,0 +1,1206 @@
+Require Import Coq.Lists.List.
+Require Import ExtLib.Structures.Functor.
+Require Import ExtLib.Structures.Applicative.
+Require Import ExtLib.Structures.Monads.
+Require Import ExtLib.Data.Member.
+Require Import ExtLib.Data.HList.
+Require Import ChargeCore.Logics.ILogic.
+Require Import ChargeCore.Tactics.Tactics.
+Require Import MirrorCore.LambdaWt.MLogic.
+Require Import MirrorCore.LambdaWt.WtExpr.
+Require Import MirrorCore.LambdaWt.SubstWt.
+Require Import MirrorCore.LambdaWt.WtMigrator.
+Require Import MirrorCore.LambdaWt.WtCtx.
+
+Set Implicit Arguments.
+Set Strict Implicit.
+
+Section simple_dep_types.
+  Variable Tsymbol : Type.
+  Variable TsymbolD : Tsymbol -> Type@{Urefl}.
+  Variable Tsymbol_eq_dec : forall a b : Tsymbol, {a = b} + {a <> b}.
+
+  Variable Esymbol : type Tsymbol -> Type.
+  Variable EsymbolD : forall t, Esymbol t -> typeD TsymbolD t.
+  Variable Esymbol_eq_dec : forall t (a b : Esymbol t), {a = b} + {a <> b}.
+
+  (** TODO(gmalecha): Move **)
+  Definition exprR tus tvs (T : Type) (R : T -> T -> Prop)
+  : exprT TsymbolD tus tvs T -> exprT TsymbolD tus tvs T -> Prop :=
+    fun v1 v2 =>
+      forall us vs, R (v1 us vs) (v2 us vs).
+
+  Definition wtRespectful {t u}
+             (P : typeD TsymbolD t -> typeD TsymbolD t -> Prop)
+             (Q : typeD TsymbolD u -> typeD TsymbolD u -> Prop)
+  : typeD TsymbolD (TArr t u) -> typeD TsymbolD (TArr t u) -> Prop :=
+    fun f g => forall x y, P x y -> Q (f x) (g y).
+
+  Lemma exprR_Ap_exprT
+  : forall tus tvs (T U : type Tsymbol) P Q
+           (f g : exprT TsymbolD tus tvs (typeD TsymbolD (TArr T U)))
+           (x y : exprT TsymbolD tus tvs (typeD TsymbolD T)),
+      exprR (wtRespectful P Q) f g ->
+      exprR P x y ->
+      exprR Q (Ap_exprT f x) (Ap_exprT g y).
+  Proof using.
+    clear.
+    unfold wtRespectful, Ap_exprT, exprR.
+    intros; eauto.
+  Defined.
+
+
+  Context (Inst : list _ -> Type)
+          {Inst_Inst : Instantiation TsymbolD Esymbol Inst}.
+
+  Variable tyProp : type Tsymbol.
+  Context {tyPropL : ILogicOps (typeD TsymbolD tyProp)}.
+  Context {tyPropLo : ILogic (typeD TsymbolD tyProp)}.
+
+  Section hlist_maps.
+    Context {T U : Type} (f : T -> U) (F : U -> Type).
+
+    Fixpoint hlist_to_hlist_map ls (hs : hlist (fun x => F (f x)) ls)
+    : hlist F (map f ls) :=
+      match hs in hlist _ ls
+            return hlist F (map f ls)
+      with
+      | Hnil => Hnil
+      | @Hcons _ _ x xs h hs =>
+        @Hcons _ _ (f x) (map f xs) h (@hlist_to_hlist_map _ hs)
+      end.
+  End hlist_maps.
+
+  Section logicM.
+
+    Fixpoint foralls_prop (ts : list (type Tsymbol))
+    : (hlist (typeD TsymbolD) ts -> typeD TsymbolD tyProp) ->
+      typeD TsymbolD tyProp :=
+      match ts with
+      | nil => fun k => k Hnil
+      | t :: ts => fun k =>
+        foralls_prop (fun vs =>
+                        lforall (fun v => k (Hcons v vs)))
+      end.
+
+    Fixpoint foralls_uvar_prop (ts : list (Tuvar Tsymbol))
+    : (hlist (fun tst => hlist (typeD TsymbolD) (fst tst) -> typeD TsymbolD (snd tst)) ts -> Prop) ->
+      Prop :=
+      match ts with
+      | nil => fun k => k Hnil
+      | t :: ts => fun k =>
+        foralls_uvar_prop (fun vs => forall v, k (Hcons v vs))
+      end.
+
+    Section impls.
+      Context {tus : list (Tuvar Tsymbol)} {tvs : list (type Tsymbol)}.
+      Fixpoint impls_prop (ts : list (typeD TsymbolD tyProp))
+               (post : typeD TsymbolD tyProp)
+      : typeD TsymbolD tyProp :=
+        match ts with
+        | nil => post
+        | t :: ts =>
+          limpl t (impls_prop ts post)
+        end.
+    End impls.
+
+    Variable m : Type -> Type.
+
+    Arguments wtctx [_] _ _ _ _.
+
+    (** TODO(gmalecha):
+     **  I need to figure out how contexts should play into this.
+     **  - Should [tus] and [tvs] be computed from the context, or should
+     **    the type of contexts be dependent on them?
+     **)
+    Record resultA tus resultUs T : Type := mkResultA
+    { result         : T (*
+      (** The only reason to return this is to avoid duplicate work
+       ** when doing migration.
+       **)
+    ; resultPrems    : wtctx Esymbol tyProp resultUs tvs *)
+    ; resultSubst    : Inst resultUs
+    ; resultMigrator : migrator Esymbol tus resultUs }.
+    Arguments mkResultA {_ _ _} _ _ _ : clear implicits.
+
+    Record resultC tus T : Type := mkResultC
+    { resultUs       : _
+    ; the_result     : resultA tus resultUs T }.
+    Arguments mkResultC {_ _} _ _ : clear implicits.
+
+    (** Statically known pre- and post-context
+     **)
+    Definition InCtxA tus tus' tvs (T : Type) : Type :=
+      forall (sub : Inst tus) (ctx : wtctx Esymbol tyProp tus tvs),
+        m (resultA tus tus' T).
+
+    (** Statically known pre- context
+     **)
+    Definition InCtxC tus tvs (T : Type) : Type :=
+      forall (sub : Inst tus) (ctx : wtctx Esymbol tyProp tus tvs),
+        m (resultC tus T).
+
+    (* (** NOTE: [logicT] does not form a monad due to the generalization *)
+    (*  **       over the indices. *)
+    (*  **) *)
+    (* Definition logicM : Type := *)
+    (*   forall tus tvs, logicC tus tvs. *)
+
+    (* Variable PreD *)
+    (* : forall {tus tvs}, Pre tus tvs -> *)
+    (*                     exprT TsymbolD tus tvs (typeD TsymbolD tyProp). *)
+    (* Variable PostD *)
+    (* : forall {tus tvs}, Post tus tvs -> *)
+    (*                     exprT TsymbolD tus tvs (typeD TsymbolD tyProp). *)
+
+    Context {Functor_m : Functor m}.
+    Context {FLogic_m : FLogic m}.
+
+    Arguments wtctxD [_ _ _] _ _ {_} [_ _] _ _ _ _.
+
+    Global Instance ILogicOps_exprT T (ILo : ILogicOps T) tus tvs
+    : ILogicOps (exprT TsymbolD tus tvs T) :=
+    { lentails := fun P Q => forall us vs, P us vs |-- Q us vs
+    ; ltrue    := fun _ _ => ltrue
+    ; lfalse   := fun _ _ => lfalse
+    ; land     := fun P Q us vs => P us vs //\\ Q us vs
+    ; lor      := fun P Q us vs => P us vs \\// Q us vs
+    ; limpl    := fun P Q us vs => P us vs -->> Q us vs
+    ; lforall  := fun T P us vs => lforall (fun x => P x us vs)
+    ; lexists  := fun T P us vs => lexists (fun x => P x us vs)
+    }.
+    Global Instance ILogic_exprT T (ILo : ILogicOps T) (IL : ILogic T) tus tvs
+    : ILogic (exprT TsymbolD tus tvs T).
+    Proof using.
+      clear - IL.
+      constructor; try red; simpl; intros.
+      { constructor.
+        { red. reflexivity. }
+        { red. intros. etransitivity; [ eapply H | eapply H0 ]. } }
+      { eapply ltrueR. }
+      { eapply lfalseL. }
+      { eapply lforallL; eapply H. }
+      { eapply lforallR. intros. eapply H. }
+      { eapply lexistsL. eauto. }
+      { eapply lexistsR. eapply H. }
+      { eapply landL1; eapply H. }
+      { eapply landL2; eapply H. }
+      { eapply lorR1; eapply H. }
+      { eapply lorR2; eapply H. }
+      { eapply landR; [ eapply H | eapply H0 ]. }
+      { eapply lorL; [ eapply H | eapply H0 ]. }
+      { eapply landAdj. apply H. }
+      { eapply limplAdj. apply H. }
+    Defined.
+
+    Require Import ChargeCore.Logics.ILEmbed.
+    Global Instance EmbedOp_Prop_tyProp : EmbedOp Prop (typeD TsymbolD tyProp).
+    Admitted.
+    Global Instance Embed_Prop_tyProp : Embed Prop (typeD TsymbolD tyProp).
+    Admitted.
+    Global Instance EmbedOp_UProp_tyProp {tus tvs}
+    : EmbedOp (Uenv TsymbolD tus -> Prop)
+              (exprT TsymbolD tus tvs (typeD TsymbolD tyProp)) :=
+    { embed := fun P us _ => embed (P us) }.
+(*
+    Global Instance Embed_UProp_tyProp {tus tvs}
+    : Embed (Uenv TsymbolD tus -> Prop)
+            (exprT TsymbolD tus tvs (typeD TsymbolD tyProp)).
+    { embed := fun P us _ => embed (P us) }.
+*)
+
+    (** This basically says that the second is equal to the migration of the
+     ** first. It is only important if I have delayed migration of contexts.
+     **)
+    Axiom wtctx_migrates : forall {tus tus' tvs}, migrator Esymbol tus tus' ->
+        wtctx Esymbol tyProp tus tvs -> wtctx Esymbol tyProp tus' tvs -> Prop.
+
+    Arguments WtMigrator.vars_id {_ _ _ _}.
+    Arguments wtgoal_subst {_ _ _ _ _} _ [_ _] _ _.
+
+    (** This is an eager migration function **)
+    Fixpoint migrate_wtctx {tus tus' tvs} (mig : migrator Esymbol tus tus')
+             (ctx : wtctx Esymbol tyProp tus tvs)
+    : wtctx Esymbol tyProp tus' tvs :=
+      match ctx in wtctx _ _ _ tvs return wtctx Esymbol tyProp tus' tvs with
+      | ctx_Top => ctx_Top
+      | ctx_All t c => ctx_All t (migrate_wtctx mig c)
+      | ctx_Hyp P c => ctx_Hyp (migrate_expr mig P) (migrate_wtctx mig c)
+(*
+      | ctx_Left G c =>
+        ctx_Left (wtgoal_subst mig WtMigrator.vars_id G)
+                 (migrate_wtctx mig c)
+      | ctx_Right G c =>
+        ctx_Right (wtgoal_subst mig WtMigrator.vars_id G)
+                  (migrate_wtctx mig c)
+*)
+      end.
+
+    Definition InCtxA_spec {tus tus' tvs T} (c : InCtxA tus tus' tvs T)
+               (TD : T -> exprT TsymbolD tus' tvs (typeD TsymbolD tyProp))
+    : Prop :=
+      forall sub ctx,
+        fmodels (fun t =>
+                   match t with
+                   | mkResultA val sub' mig =>
+                     let ctx' := migrate_wtctx mig ctx in
+                     Inst_evolves mig sub sub' /\
+(*                     wtctx_migrates mig ctx ctx' /\ *)
+                         (embed (InstD sub'))
+                     |-- (wtctxD EsymbolD tyProp ctx'
+                                 (fun us vs => TD val us vs))
+                   end)
+                (c sub ctx).
+
+    Context {Monad_m : Monad m}.
+
+    Global Instance Monad_WtInCtx {tus tvs} : Monad (InCtxA tus tus tvs) :=
+    { ret := fun T val sub ctx => ret {| result := val
+                                       ; resultSubst := sub
+                                       ; resultMigrator := migrator_id |}
+    ; bind := fun _ _ c k sub ctx =>
+                bind (c sub ctx)
+                     (fun val =>
+                        match val with
+                        | mkResultA val sub' mig =>
+                          k val sub' (migrate_wtctx mig ctx)
+                        end)
+    }.
+    Global Instance Functor_WtInCtx {tus tus' tvs} : Functor (InCtxA tus tus' tvs) :=
+    { fmap := fun T U f x sub ctx =>
+                fmap (fun val =>
+                        match val with
+                        | mkResultA val sub mig =>
+                          mkResultA (f val) sub mig
+                        end) (x sub ctx) }.
+
+    Context {MLogic_m : MLogic m}.
+
+(*
+    Definition logicC_spec {tus tvs} (c : logicC tus tvs) : Prop :=
+      forall prems goal inst result,
+        c prems inst goal = result ->
+        fmodels (fun t =>
+              match t with
+              | @mkResultC _ _ tus' (mkResultA post prems' inst' trans) =>
+                Inst_evolves trans inst inst' /\
+                @foralls_uvar_prop tus' (fun us' =>
+                  let us := migrate_env EsymbolD trans us' in
+                  InstD inst' us' ->
+                  lentails ltrue
+                    (@foralls_prop tvs (fun vs =>
+                       limpl (impls_prop
+                                (map (fun p => wtexprD EsymbolD p us' vs) prems')
+                                (@PostD _ _ post us' vs))
+                             (impls_prop
+                                (map (fun p => wtexprD EsymbolD p us vs) prems)
+                                (@PreD  _ _ goal us  vs)))))
+              end)
+           result.
+
+    Definition logicM_spec (l : logicM) : Prop :=
+      forall tus tvs,
+        logicC_spec (l tus tvs).
+*)
+  End logicM.
+
+  Lemma foralls_uvar_prop_impl
+    : forall ts (P Q : _ -> Prop),
+      (forall xs, P xs -> Q xs) ->
+      (@foralls_uvar_prop ts P -> @foralls_uvar_prop ts Q).
+  Proof.
+    clear.
+    induction ts; simpl; intros; auto.
+    eapply IHts; [| eassumption ].
+    simpl. eauto.
+  Qed.
+
+  Lemma foralls_prop_impl : forall ts P Q,
+      (forall xs, P xs |-- Q xs) ->
+      @foralls_prop ts P |-- @foralls_prop ts Q.
+  Proof.
+    clear - tyPropLo.
+    induction ts; simpl; eauto.
+    intros.
+    eapply IHts. intros.
+    eapply lforallR. intros. eapply lforallL. eapply H.
+  Qed.
+
+  Lemma foralls_uvar_prop_sem
+    : forall ts (P : _ -> Prop),
+      (forall xs, P xs) ->
+      (@foralls_uvar_prop ts P).
+  Proof.
+    clear.
+    induction ts; simpl; intros; auto.
+  Qed.
+
+  Lemma foralls_prop_sem : forall ts Q,
+      (forall xs, |-- Q xs) ->
+      |-- @foralls_prop ts Q.
+  Proof.
+    clear - tyPropLo.
+    induction ts; simpl; eauto.
+    intros.
+    eapply IHts. intros.
+    eapply lforallR. intros. eauto.
+  Qed.
+
+  Lemma impls_prop_pure : forall A B,
+      A |-- B ->
+      forall Cs,
+        A |-- impls_prop Cs B.
+  Proof.
+    induction Cs; simpl; intros; eauto.
+    apply limplAdj.
+    etransitivity; [ | eapply IHCs ].
+    eapply landL1. reflexivity.
+  Qed.
+
+
+  Section evar_tactic.
+    Context {m : Type -> Type}.
+    Context {Monad_m : Monad m}.
+    Context {Functor_m : Functor m}.
+    Context {FLogic_m : FLogic m}.
+    Context {MLogic_m : MLogic m}.
+
+    Variables Pre Post Post'
+    : list (Tuvar Tsymbol) -> list (type Tsymbol) -> Type.
+    Variable Pre_migrate
+    : forall tus t tvs, migrator Esymbol tus (tus ++ t :: nil) ->
+                        Pre tus tvs -> Pre (tus ++ t :: nil) tvs.
+
+    Arguments DepUtil.member_weaken {_} [_] _ [_] _.
+
+    Definition Evar {tus tvs} t
+    : InCtxA m tus (tus ++ t :: nil) tvs (member t (tus ++ t :: nil)) :=
+      fun sub _ =>
+        let mig := migrator_fresh t tus in
+        ret {| result := DepUtil.member_weaken tus (MZ _ _)
+(*             ; resultPrems := map (migrate_expr mig) prems *)
+             ; resultSubst := Inst_fresh t sub
+             ; resultMigrator := mig |}.
+
+(*
+    Fixpoint build_evars T (tus' : list (Tuvar Tsymbol)) (k : forall t X, member t X -> T X t) {struct tus'}
+    : hlist (T tus') tus' :=
+      match tus' as tus'
+            return hlist (T tus') tus'
+      with
+      | nil => Hnil
+      | t :: tus' =>
+        Hcons (k _ _ (MZ _ _))
+              (build_evars (fun X t' => T (t :: X) t') tus' (fun _ _ m => k _ _ (MN _ m)))
+      end.
+*)
+
+    Definition InCtxA_pure {tus tvs} {T : Type} (x : T)
+    : InCtxA m tus tus tvs T :=
+      fun sub _ =>
+        ret {| result      := x
+             ; resultSubst := sub
+             ; resultMigrator := migrator_id |}.
+
+    Definition InCtxA_bind {tus tus' tus'' tvs} {T U}
+               (x : InCtxA m tus tus' tvs T)
+               (k : T -> InCtxA m tus' tus'' tvs U)
+    : InCtxA m tus tus'' tvs U :=
+      fun sub ctx =>
+        bind (x sub ctx)
+             (fun x =>
+                let ctx' := migrate_wtctx x.(resultMigrator) ctx in
+                bind (k x.(result) x.(resultSubst) ctx')
+                     (fun r =>
+                        ret {| result := r.(result)
+                             ; resultSubst := r.(resultSubst)
+                             ; resultMigrator := migrator_compose x.(resultMigrator) r.(resultMigrator) |})).
+
+    (** This is really inefficient due to all of the casting *)
+    Fixpoint Evars {tus tvs} tus'
+    : InCtxA m tus (tus ++ tus') tvs (hlist (fun t => member t (tus ++ tus')) tus') :=
+      match tus' as tus'
+            return InCtxA m tus (tus ++ tus') tvs (hlist (fun t => member t (tus ++ tus')) tus')
+      with
+      | nil =>
+        match eq_sym (app_nil_r_trans tus) in _ = X
+              return InCtxA m tus X tvs (hlist (fun t => member t X) nil)
+        with
+        | eq_refl => InCtxA_pure Hnil
+        end
+      | t :: tus' =>
+        InCtxA_bind (Evar t)
+                    (fun u =>
+                       match app_ass_trans tus (t :: nil) tus' in _ = X
+                             return InCtxA m (tus ++ t :: nil) X tvs (hlist (fun t0 : Tuvar Tsymbol => member t0 X) (t :: tus'))
+                       with
+                       | eq_refl =>
+                         fmap (fun us =>
+                                 Hcons match app_nil_r_trans tus' in _ = Y
+                                             return member t (_ ++ Y)
+                                       with
+                                       | eq_refl => @DepUtil.member_lift _ t nil tus' (tus ++ t :: nil)
+                                                                         (match app_nil_r_trans (tus ++ t :: nil) in _ = X
+                                                                                return member t X -> member t _
+                                                                          with
+                                                                          | eq_refl => fun x => x
+                                                                          end u)
+                                       end us) (Evars tus')
+                              end)
+      end.
+
+  End evar_tactic.
+
+  Require Import MirrorCore.LambdaWt.Unify.
+
+  Section apply_tactic.
+    Variable m : Type -> Type.
+    Context {Monad_m : Monad m}.
+    Context {MonadZero_m : MonadZero m}.
+    Context {Functor_m : Functor m}.
+
+    Context {FLogic_m : FLogic m}.
+    Context {MLogic_m : MLogic m}.
+    Context {MLogicZero_m : MLogicZero m}.
+
+    Variable unify : Unifier Esymbol Inst.
+    Variable unifyOk : UnifierOk unify.
+
+    Section lemma.
+      Variable C : list (Tuvar Tsymbol) -> list (type Tsymbol) -> Type.
+      Variable CD : forall {tus tvs},
+          C tus tvs -> exprT TsymbolD tus tvs (typeD TsymbolD tyProp).
+
+      Record lemma tus tvs : Type :=
+      { vars  : list (type Tsymbol)
+      ; premises : list (wtexpr Esymbol tus (vars ++ tvs) tyProp)
+      ; concl : C tus (vars ++ tvs)
+      }.
+
+      Definition lemmaD {tus tvs} (l : lemma tus tvs)
+      : exprT TsymbolD tus tvs (typeD TsymbolD tyProp) :=
+        fun us vs =>
+          foralls_prop
+            (fun vs' : Venv TsymbolD l.(vars) =>
+               impls_prop
+                 (map (fun e => wtexprD EsymbolD e us (hlist_app vs' vs))
+                      l.(premises))
+                 (CD l.(concl) us (hlist_app vs' vs))).
+
+      Definition lift_lemma {tus tvs} {tus'} tvs'
+                 (mig : migrator Esymbol tus tus')
+                 (lem : lemma tus tvs)
+      : lemma tus' (tvs' ++ tvs).
+      Proof using.
+      Admitted.
+
+      Global Instance Migrate_lemma : Migrate Esymbol lemma.
+      Admitted.
+    End lemma.
+
+    Arguments lift_lemma {_ _ _ _} _ _ _.
+    About Evars.
+    Arguments Evars {_ _ _} [_ _] _ _ _.
+    Arguments migrate_expr {_ _} [_ _] _ [_ _] _.
+
+    (** Soundness of unification should be justified once! *)
+    Definition Unify {tus tvs t}
+               (e1 e2 : wtexpr Esymbol tus tvs t)
+    : InCtxA m tus tus tvs bool :=
+      fun sub ctx =>
+        match unify e1 e2 sub
+              return m (resultA tus tus bool)
+        with
+        | None =>
+          ret (m:=m)
+              {| result := false
+               ; resultSubst := sub
+               ; resultMigrator := migrator_id
+               |}
+        | Some sub' =>
+          ret {| result := true
+               ; resultSubst := sub'
+               ; resultMigrator := migrator_id
+               |}
+        end.
+
+    (** TODO(gmalecha): move this to WtMigrator *)
+    Definition migrator_pure {tus}
+    : migrator Esymbol nil tus := Hnil.
+
+    Definition inj_lemma {tus tvs}
+               (lem : lemma (fun tus tvs => wtexpr Esymbol tus tvs tyProp) nil nil)
+    : InCtxA m tus tus tvs (lemma (fun tus tvs => wtexpr Esymbol tus tvs tyProp) tus tvs) :=
+      InCtxA_pure (
+               match app_nil_r_trans tvs in _ = X return lemma _ _ X with
+               | eq_refl => lift_lemma tvs (@migrator_pure tus) lem
+               end).
+
+    Arguments WtMigrator.vars_id {_ _ _ _}.
+
+    Definition InCtxA_listen_migrator {tus tus' tvs T}
+               (c : InCtxA m tus tus' tvs T)
+    : InCtxA m tus tus' tvs (T * migrator Esymbol tus tus') :=
+      fun sub ctx =>
+        bind (c sub ctx)
+             (fun x => ret {| result := (x.(result), x.(resultMigrator))
+                            ; resultSubst := x.(resultSubst)
+                            ; resultMigrator := x.(resultMigrator) |}).
+
+    Require Import ExtLib.Data.List.
+    Instance MonadZero_InCtxA {tus tus' tvs}
+    : MonadZero (InCtxA m tus tus' tvs) :=
+    {| mzero := fun _ _ _ => mzero |}.
+
+    Section hlist_strong_map.
+      Context {T U : Type} {f : T -> U} {F : T -> Type} {G : U -> Type}
+              (FG : forall x, G (f x) -> F x).
+      Fixpoint hlist_strong_map {ls}
+      : hlist G (map f ls) -> hlist F ls :=
+        match ls as ls return hlist G (map f ls) -> hlist F ls with
+        | nil => fun _ => Hnil
+        | l :: ls => fun h => Hcons (FG (hlist_hd h)) (hlist_strong_map (hlist_tl h))
+        end.
+    End hlist_strong_map.
+
+    Definition EApply {tus tvs}
+               (lem : lemma (fun tus tvs => wtexpr Esymbol tus tvs tyProp)
+                            tus tvs)
+               (gl : wtexpr Esymbol tus tvs tyProp)
+    : InCtxA m tus (tus ++ List.map (fun t => (tvs,t)) lem.(vars)) tvs
+             (list (wtexpr Esymbol (tus ++ List.map (fun t => (tvs,t)) lem.(vars)) tvs tyProp)).
+    refine
+      (let vs := List.map (fun t => (tvs,t)) lem.(vars) in
+       InCtxA_bind (InCtxA_listen_migrator (Evars vs))
+                   (fun us =>
+                      let x : migrator Esymbol tus (tus ++ vs) := snd us in
+                      let new_us : hlist (wtexpr Esymbol (tus ++ vs) tvs) (vars lem) :=
+                          hlist_strong_map (fun _ X => wtUVar X WtMigrator.vars_id)
+                                           (fst us)
+                      in
+                      let lem_migrator : forall t, wtexpr Esymbol tus (lem.(vars) ++ tvs) t ->
+                                                   wtexpr Esymbol (tus ++ vs) tvs t
+                          := (* subst (hlist_app new_us WtMigrator.vars_id) gl' *)
+                          (* migrate_expr x lem.(concl) *) _
+                      in
+                      InCtxA_bind (Unify (migrate_expr x gl) (lem_migrator _ lem.(concl)))
+                                  (fun x => if x then
+                                              ret (fmap (lem_migrator tyProp) lem.(premises))
+                                            else mzero))).
+    intros.
+    generalize (migrate_expr x X).
+    eapply subst.
+    eapply hlist_app.
+    2: eapply WtMigrator.vars_id.
+    eapply new_us.
+    Defined.
+
+  End apply_tactic.
+
+  Lemma wtexpr_equiv_Unifiable_eq
+  : forall tus tvs t (e1 e2 : wtexpr Esymbol tus tvs t)
+           (i : Inst tus),
+      wtexpr_equiv (Unifiable_eq i) e1 e2 ->
+      forall (xs : Uenv TsymbolD tus)
+             (vs : Venv TsymbolD tvs),
+        InstD i xs ->
+        wtexprD EsymbolD e1 xs vs = wtexprD EsymbolD e2 xs vs.
+  Proof.
+    induction 1; intros; try solve [ eauto | eapply H; eapply H0 ].
+    { simpl.
+      unfold Ap_exprT.
+      rewrite IHwtexpr_equiv1; eauto.
+      rewrite IHwtexpr_equiv2; eauto. }
+    { simpl. unfold Abs_exprT.
+      eapply FunctionalExtensionality.functional_extensionality; eauto. }
+    { simpl. unfold UVar_exprT.
+      repeat rewrite hlist_map_hlist_map.
+      f_equal.
+      clear - H0 H.
+      induction H; simpl; auto.
+      f_equal; eauto. }
+    { destruct pf.
+      { inversion H0; clear H0; subst.
+        (** TODO(gmalecha): This should be provable *)
+        admit. }
+      { inversion H0; clear H0; subst.
+        (** TODO(gmalecha): This should be provable *)
+        admit. } }
+    { etransitivity;
+      [ eapply IHwtexpr_equiv1 | eapply IHwtexpr_equiv2 ]; eauto. }
+  Admitted.
+
+
+  Section assumption_tactic.
+    Variable m : Type -> Type.
+    Context {Monad_m : Monad m}.
+    Context {MonadPlus_m : MonadPlus m}.
+    Context {MonadZero_m : MonadZero m}.
+    Context {Functor_m : Functor m}.
+
+    Variable unify : Unifier Esymbol Inst.
+    Variable unifyOk : UnifierOk unify.
+
+    Context {FLogic_m : FLogic m}.
+    Context {MLogic_m : MLogic m}.
+    Context {MLogicPlus_m : MLogicPlus m}.
+    Context {MLogicZero_m : MLogicZero m}.
+
+    Fixpoint member_lower {T : Type} {t : T} {ts ts'} : member t (ts' ++ ts) -> option (member t ts) :=
+      match ts' as ts'
+            return member t (ts' ++ ts) -> option (member t ts)
+      with
+      | nil => Some
+      | t' :: ts' => fun m =>
+                       match m in member _ TS
+                             return (member t (tl TS) -> option (member t ts)) -> option (member t ts)
+                       with
+                       | MZ _ _ => fun _ => None
+                       | MN _ m => fun f => f m
+                       end (fun m => @member_lower T t ts ts' m)
+      end.
+
+    Fixpoint member_skip {T : Type} {t : T} {ts ts' ts''} (f : member t ts -> option (member t ts''))
+             {struct ts'}
+    : member t (ts' ++ ts) -> option (member t (ts' ++ ts'')).
+    refine
+      match ts' as ts'
+            return member t (ts' ++ ts) -> option (member t (ts' ++ ts''))
+      with
+      | nil => f
+      | t' :: ts' => fun m =>
+        match m in member _ (T :: TS)
+              return T = t' -> (member t TS -> option (member t (ts' ++ ts''))) -> _
+        with
+        | MZ _ _ => fun pf _ => Some (MZ _ _)
+        | MN _ m => fun pf f => fmap (@MN _ _ _ _) (f m)
+        end eq_refl (fun m => member_skip _ _ _ _ _ f m)
+      end.
+    Defined.
+
+    Fixpoint wtexpr_lower {tus} tvs tvs' tvs'' t (e : wtexpr Esymbol tus (tvs'' ++ tvs' ++ tvs) t)
+    : option (wtexpr Esymbol tus (tvs'' ++ tvs) t).
+    refine
+      (match e in wtexpr _ _ _ t
+             return option (wtexpr Esymbol tus (tvs'' ++ tvs) t)
+       with
+       | wtVar m => fmap (@wtVar _ _ _ _ _) (member_skip (ts':= tvs'') (member_lower) m)
+       | wtApp f x => match wtexpr_lower tus tvs tvs' tvs'' _ f
+                          , wtexpr_lower tus tvs tvs' tvs'' _ x
+                      with
+                      | Some f' , Some x' => Some (wtApp f' x')
+                      | _ , _ => None
+                      end
+       | wtInj x => Some (wtInj x)
+       | wtAbs e => fmap (@wtAbs _ _ _ _ _ _) (wtexpr_lower tus tvs tvs' (_ :: tvs'') _ e)
+       | wtUVar u es =>
+         fmap (wtUVar u) _
+       end).
+    admit.
+    Admitted.
+
+    Section find_premise_ctx.
+      Context {tus : list (Tuvar Tsymbol)}.
+      Variables (s : Inst tus).
+
+
+      Fixpoint find_premise_ctx {tvs tvs'}
+               (ctx : wtctx _ Esymbol tyProp tus tvs)
+      : wtexpr Esymbol tus (tvs' ++ tvs) tyProp -> m (Inst tus) :=
+        match ctx in wtctx _ _ _ _ tvs
+               return wtexpr Esymbol tus (tvs' ++ tvs) tyProp -> m (Inst tus)
+         with
+         | ctx_Top => fun _ => mzero
+         | ctx_All t ctx' => fun x =>
+           @find_premise_ctx _ (tvs' ++ t::nil) ctx'
+                             match eq_sym (app_ass_trans tvs' (t::nil) _) in _ = X
+                                   return wtexpr Esymbol tus X tyProp
+                             with
+                             | eq_refl => x
+                             end
+         | ctx_Hyp P ctx' => fun gl =>
+           match @wtexpr_lower _ _ _ nil _ gl with
+           | None => mzero
+           | Some gl' =>
+             match unify P gl' s with
+             | None => @find_premise_ctx _ nil ctx' gl'
+             | Some s' => ret s'
+             end
+           end
+(*
+         | ctx_Left _ ctx' => fun x => find_premise_ctx ctx' x
+         | ctx_Right _ ctx' => fun x => find_premise_ctx ctx' x
+*)
+         end.
+
+      Arguments wtctxD {_ _ _} _ _ {_} [_ _] _ _ _ _ : clear implicits.
+
+      Local Lemma find_premise_ctx_sound {tvs}
+      : forall ctx tvs' gl,
+          fmodels (fun inst' : Inst tus =>
+                let trans := migrator_id in
+                Inst_evolves trans s inst' /\
+                foralls_uvar_prop
+                  (fun
+                      us : hlist
+                             (fun tst : list (type Tsymbol) * type Tsymbol =>
+                                hlist (typeD TsymbolD) (fst tst) -> typeD TsymbolD (snd tst))
+                             tus =>
+                      InstD inst' us ->
+                      lentails ltrue
+                               (wtctxD EsymbolD tyProp ctx
+                                       (fun us vs => lforall (fun vs' => wtexprD EsymbolD gl us (hlist_app vs' vs)))
+                                       us Hnil)))
+             (@find_premise_ctx tvs tvs' ctx gl).
+      Proof.
+        induction ctx; simpl; intros.
+        { eapply fmodels_mzero. }
+        { lazymatch goal with
+          | |- fmodels _ (find_premise_ctx _ ?X) =>
+            generalize (IHctx (tvs' ++ t :: nil) X); clear IHctx
+          end.
+          eapply fmodels_conseq; simpl; intros.
+          destruct H; split; [ assumption | ].
+          revert H0.
+          eapply foralls_uvar_prop_impl; intros.
+          rewrite (H0 H1).
+          clear H0 H1.
+          admit. }
+        { Require Import ExtLib.Tactics.
+          consider (wtexpr_lower ts tvs' nil gl).
+          { admit. }
+          { intros. eapply fmodels_mzero. } }
+(*
+        { generalize (IHctx _ gl).
+          eapply fmodels_conseq; simpl; intros.
+          destruct H; split; [ eassumption | ].
+          revert H0.
+          eapply foralls_uvar_prop_impl; intros.
+          specialize (H0 H1).
+          rewrite H0.
+          admit. }
+        { generalize (IHctx _ gl).
+          eapply fmodels_conseq; simpl; intros.
+          destruct H; split; [ eassumption | ].
+          revert H0.
+          eapply foralls_uvar_prop_impl; intros.
+          specialize (H0 H1).
+          rewrite H0.
+          admit. }
+*)
+      Admitted.
+
+    End find_premise_ctx.
+
+    Section find_premise.
+      Context {tus : list (Tuvar Tsymbol)}.
+      Context {tvs : list (type Tsymbol)}.
+      Variables (gl : wtexpr Esymbol tus tvs tyProp)
+                (s : Inst tus).
+
+      Fixpoint find_premise
+               (prems : list (wtexpr Esymbol tus tvs tyProp))
+      : m (Inst tus) :=
+        match prems with
+        | nil => mzero
+        | p :: ps =>
+          match @unify _ _ _ gl p s with
+          | None => find_premise ps
+          | Some s' => mjoin (ret s') (find_premise ps)
+          end
+        end.
+
+      Local Lemma find_premise_sound
+      : forall prems,
+          fmodels (fun inst' : Inst tus =>
+                let trans := migrator_id in
+                Inst_evolves trans s inst' /\
+                foralls_uvar_prop
+                  (fun
+                      us : hlist
+                             (fun tst : list (type Tsymbol) * type Tsymbol =>
+                                hlist (typeD TsymbolD) (fst tst) -> typeD TsymbolD (snd tst))
+                             tus =>
+                      InstD inst' us ->
+                      lentails ltrue
+                        (foralls_prop
+                                      (fun vs : hlist (typeD TsymbolD) tvs =>
+                                         impls_prop
+                                                    (map
+                                                       (fun p : wtexpr Esymbol tus tvs tyProp =>
+                                                          wtexprD EsymbolD p us vs) prems)
+                                                    (wtexprD EsymbolD gl us vs)))))
+             (find_premise prems).
+      Proof.
+        induction prems.
+        { eapply fmodels_mzero. }
+        { simpl.
+          lazymatch goal with
+          | |- fmodels ?X _ =>
+            assert (fmodels X (find_premise prems))
+          end.
+          { revert IHprems; eapply fmodels_conseq.
+            simpl. destruct 1; split; auto.
+            revert H0.
+            eapply foralls_uvar_prop_impl.
+            intros.
+            etransitivity; [ eapply H0; eassumption | ].
+            eapply foralls_prop_impl; intros.
+            eapply limplAdj. eapply landL1. reflexivity. }
+          clear IHprems.
+          destruct (unify gl a s) eqn:?; eauto.
+          eapply fmodels_mjoin; [ | solve [ eauto ] ].
+          clear H.
+          eapply fmodels_ret.
+          eapply unifyOk in Heqo.
+          destruct Heqo; split; [ eassumption | ].
+          eapply foralls_uvar_prop_sem. intros.
+          eapply foralls_prop_sem; intros.
+          eapply limplAdj.
+          eapply impls_prop_pure.
+          eapply landL2.
+          erewrite <- wtexpr_equiv_Unifiable_eq; eauto.
+          { reflexivity. } }
+      Qed.
+
+    End find_premise.
+
+
+    Lemma impls_prop_ap
+      : forall P Q prems G,
+        G |-- impls_prop prems (P -->> Q) ->
+        G |-- impls_prop prems P -->> impls_prop prems Q.
+    Proof.
+      induction prems; simpl; auto.
+      intros.
+      charge_intros.
+      charge_eapply (IHprems (G //\\ a)).
+      charge_split.
+      { charge_tauto. }
+      { charge_tauto. }
+      Unshelve.
+      charge_tauto.
+    Qed.
+
+    Definition Assumption {tus tvs}
+               (gl : wtexpr Esymbol tus tvs tyProp)
+    : InCtxA m tus tus tvs unit :=
+      fun sub ctx =>
+        fmap (F:=m)
+             (fun sub' => mkResultA tt sub' migrator_id)
+             (find_premise_ctx sub (tvs':=nil) ctx gl).
+
+    Theorem foralls_uvar_prop_sem'
+      : forall (ts : list (Tuvar Tsymbol))
+               (P : hlist
+                      (fun tst : list (type Tsymbol) * type Tsymbol =>
+                         hlist (typeD TsymbolD) (fst tst) -> typeD TsymbolD (snd tst))
+                      ts -> Prop),
+        foralls_uvar_prop P ->
+        (forall
+            xs : hlist
+                   (fun tst : list (type Tsymbol) * type Tsymbol =>
+                      hlist (typeD TsymbolD) (fst tst) -> typeD TsymbolD (snd tst))
+                   ts, P xs).
+    Proof.
+      induction ts; simpl.
+      { intros. rewrite (hlist_eta xs). apply H. }
+      { intros. rewrite (hlist_eta xs).
+        eapply IHts in H. eapply H. }
+    Qed.
+
+    Theorem Assumption_sound {tus tvs} gl
+    : InCtxA_spec (@Assumption tus tvs gl)
+                  (fun _ => wtexprD EsymbolD gl).
+    Proof.
+      red. unfold Assumption. intros.
+      eapply fmodels_fmap; [ | eapply find_premise_ctx_sound ].
+      { destruct 1.
+        split; [ assumption | ].
+        red. simpl.
+        intros.
+        eapply foralls_uvar_prop_sem' in H0.
+        revert H0. instantiate (1 := us).
+        intros.
+        rewrite (hlist_eta vs).
+        rewrite <- embedPropExists'.
+        eapply lexistsL.
+        intro.
+        rewrite H0; eauto.
+        admit. }
+    Admitted.
+  End assumption_tactic.
+
+  Section cut_tactic.
+    Variable m : Type -> Type.
+    Context {Monad_m : Monad m}.
+    Context {Functor_m : Functor m}.
+
+    Context {FLogic_m : FLogic m}.
+    Context {MLogic_m : MLogic m}.
+
+    Definition Cut {tus tvs} (t gl : wtexpr Esymbol tus tvs tyProp)
+    : InCtxA m tus tus tvs (wtgoal Esymbol tyProp tus tvs)%type :=
+      fun sub ctx =>
+        ret (@mkResultA _ _ _ (wtConj (wtGoal t) (wtHyp t (wtGoal gl)))
+                        sub
+                        migrator_id).
+
+    Existing Instance Reflexive_Inst_evolves.
+
+    Arguments wtctxD [_ _ _] _ _ {_} [_ _] _ _ _ _.
+    Arguments wtctx [_] _ _ _ _.
+    Lemma wtctxD_pure
+      : forall tus tvs (ctx : wtctx Esymbol tyProp tus tvs) P,
+        |-- P ->
+        |-- wtctxD EsymbolD tyProp ctx P.
+    Proof.
+      induction ctx; simpl; intros; eauto.
+      { eapply IHctx. red; simpl.
+        intros. eapply lforallR. intros; eauto. }
+      { eapply IHctx. red; simpl.
+        intros. eapply limplAdj.
+        rewrite <- H. charge_assumption. }
+    Qed.
+
+    Theorem Cut_sound
+    : forall tus tvs t gl,
+        InCtxA_spec (@Cut tus tvs t gl)
+                    (fun gl' => wtgoalD EsymbolD gl' -->> wtexprD EsymbolD gl).
+    Proof.
+      unfold Cut. red. simpl; intros.
+      eapply fmodels_ret.
+      split; [ reflexivity | ].
+      { simpl.
+        intros.
+        charge_clear.
+        eapply wtctxD_pure.
+        red; simpl; intros.
+        charge_tauto. }
+    Qed.
+
+  End cut_tactic.
+
+End simple_dep_types.
+
+
+
+
+
+(*
+    Definition logicM_cps (Pre Post : _ -> _ -> Type) : Type :=
+      forall tus tvs
+        (prems : list (wtexpr Esymbol tus tvs tyProp))
+        (goal  : Pre tus tvs)
+        (inst  : Inst Esymbol tus)
+        (T : Type)
+        (success : forall tus' : _ ,
+            list (wtexpr Esymbol tus tvs tyProp) ->
+            Post tus' tvs ->
+            Inst Esymbol tus' ->
+            migrator tus tus' ->
+            m T)
+        (fail : unit -> m T),
+        m T.
+
+
+
+    Definition with_uvars tus (T : list (Tuvar Tsymbol) -> Type) : Type :=
+      Inst Esymbol tus ->
+      m { tus' : _ & T tus' * Inst Esymbol tus' *
+                     forall ts t, Member.member (ts,t) tus -> wtexpr Esymbol tus' ts t }%type.
+
+    Definition in_context tvs (T : Type) : Type :=
+        wtctxD
+*)
+(*
+  Section arrow_tactics.
+    Context {m : Type -> Type}.
+    Context {Monad_m : Monad m}.
+    Context {Functor_m : Functor m}.
+    Context {FLogic_m : FLogic m}.
+    Context {MLogic_m : MLogic m}.
+
+    Section pureA.
+      Variables Pre Post
+      : list (Tuvar Tsymbol) -> list (type Tsymbol) -> Type.
+
+      Definition pureA {tus tvs} (f : Pre tus tvs -> Post tus tvs)
+      : logicA m Pre Post tus tus tvs :=
+        fun prems sub goal =>
+          ret {| result := f goal
+               ; resultPrems := prems
+               ; resultSubst := sub
+               ; resultMigrator := migrator_id |}.
+
+      Variable PreD : forall tus tvs,
+          Pre tus tvs ->
+          exprT TsymbolD tus tvs (typeD TsymbolD tyProp).
+      Variable PostD : forall tus tvs,
+          Post tus tvs ->
+          exprT TsymbolD tus tvs (typeD TsymbolD tyProp).
+
+    End pureA.
+
+    Section identA.
+      Variables Pre
+      : list (Tuvar Tsymbol) -> list (type Tsymbol) -> Type.
+
+      Definition identA {tus tvs} := @pureA Pre Pre tus tvs (fun x => x).
+
+      Variable PreD : forall tus tvs,
+          Pre tus tvs ->
+          exprT TsymbolD tus tvs (typeD TsymbolD tyProp).
+
+      Theorem identA_sound
+      : forall tus tvs, logicA_spec PreD PreD (@identA tus tvs).
+      Proof.
+      Admitted.
+    End identA.
+
+    Section composeA.
+    Variables G G' G'' : list (Tuvar Tsymbol) -> list (type Tsymbol) -> Type.
+
+    Variable GD : forall tus tvs,
+        G tus tvs ->
+        exprT TsymbolD tus tvs (typeD TsymbolD tyProp).
+
+    Variable GD' : forall tus tvs,
+        G' tus tvs ->
+        exprT TsymbolD tus tvs (typeD TsymbolD tyProp).
+
+    Variable GD'' : forall tus tvs,
+        G'' tus tvs ->
+        exprT TsymbolD tus tvs (typeD TsymbolD tyProp).
+
+    Context {tus tus' tus'' : list (Tuvar Tsymbol)}.
+    Context {tvs : list (type Tsymbol)}.
+    Definition composeA
+               (a : logicA m G G' tus tus' tvs)
+               (b : logicA m G' G'' tus' tus'' tvs)
+    : logicA m G G'' tus tus'' tvs :=
+      fun prems sub goal =>
+        bind (a prems sub goal)
+             (fun x =>
+                match x with
+                | mkResultA _ goal' prems' sub' mig' =>
+                  fmap (fun x =>
+                          match x with
+                          | mkResultA _ goal'' prems'' sub'' mig'' =>
+                            mkResultA _ goal'' prems'' sub''
+                                      (migrator_compose mig' mig'')
+                          end) (b prems' sub' goal')
+                end).
+
+    Theorem composeA_sound
+    : forall a b,
+        logicA_spec GD GD' a ->
+        logicA_spec GD' GD'' b ->
+        logicA_spec GD GD'' (composeA a b).
+    Proof.
+      intros.
+      unfold composeA.
+      red; simpl; intros; subst.
+      eapply fmodels_bind.
+      { eapply H; reflexivity. }
+      { destruct x. destruct 1.
+        eapply fmodels_fmap.
+        2: eapply H0; reflexivity.
+        destruct x; destruct 1.
+        split.
+        { eapply Inst_evolves_trans; eauto. }
+        { admit. } }
+    Admitted.
+
+    Definition logicC_of_logicA (l : logicA m G G' tus tus' tvs)
+    : logicC m G G' tus tvs :=
+      fun prems sub goal =>
+        fmap (fun x => mkResultC x) (l prems sub goal).
+
+    End composeA.
+
+    Definition prodA {tus tvs} {G1 G2 G3 G4}
+               (a : logicA m G1 G2 tus tus tvs)
+               (b : logicA m G3 G4 tus tus tvs)
+    : logicA m
+             (fun tus tvs => G1 tus tvs * G3 tus tvs)%type
+             (fun tus tvs => G2 tus tvs * G4 tus tvs)%type
+             tus tus tvs :=
+      fun prems sub gl =>
+        bind (a prems sub (fst gl))
+             (fun a' =>
+                match a' with
+                | mkResultA _ gla prems' sub' mig' =>
+                  fmap (F:=m)
+                       (fun b' =>
+                          match b' with
+                          | mkResultA _ glb prems'' sub'' mig'' =>
+                            {| result := (gla,glb)
+                               ; resultPrems := prems''
+                               ; resultSubst := sub''
+                               ; resultMigrator := migrator_compose mig' mig''
+                            |}
+                          end)
+                       (b prems' sub' (snd gl))
+                      end).
+
+  End arrow_tactics.
+
+  Arguments identA {_ _ _ _ _} _ _ _.
+  Arguments composeA {_ _ _ _ _ _ _ _ _ _} _ _ _ _ _.
+  Arguments pureA {_ _ _ _ _ _} _ _ _ _.
+
+(*
+    Section migrating.
+      Context {tus tus' : list (Tuvar Tsymbol)}.
+      Context {tvs : list (type Tsymbol)}.
+
+      Context {Pre Post Val : list (Tuvar Tsymbol) -> list (type Tsymbol) -> Type}.
+      Variable migVal : Migrate Esymbol Val.
+
+      Definition migrating
+                 (c : logicA m Pre Post tus tus' tvs)
+      : logicA m
+               (fun tus tvs => Pre tus tvs * Val tus tvs)%type
+               (fun tus tvs => Post tus tvs * Val tus tvs)%type
+               tus tus' tvs :=
+        fun prems sub gl =>
+          fmap (fun x =>
+                  match x with
+                  | mkResultA _ gl' prems' sub' mig' =>
+                    mkResultA _ (gl', migrate mig' (snd gl))
+                              prems' sub' mig'
+                  end)
+               (c prems sub (fst gl)).
+    End migrating.
+*)
+
+    (** TODO(gmalecha): Fundamentally this operation is the problem.
+     ** This type does not express the fact that the lemma is related to
+     ** the outside lemma.
+     **)
+    Definition inj_lemma {tus tvs}
+               (lem : lemma (fun tus tvs => wtexpr Esymbol tus tvs tyProp) nil nil)
+    : logicA m
+             (fun tus tvs => unit)
+             (fun tus tvs => lemma (fun tus tvs => wtexpr Esymbol tus tvs tyProp) tus tvs)
+             tus tus tvs :=
+      pureA (fun _ =>
+               match app_nil_r_trans tvs in _ = X return lemma _ _ X with
+               | eq_refl => lift_lemma tvs (@migrator_pure tus) lem
+               end).
+
+    Definition Var {tus tvs} {t} (mem : member t tvs)
+    : logicA m
+             (fun _ _ => unit)
+             (fun tus tvs => wtexpr Esymbol tus tvs t)
+             tus tus tvs :=
+      pureA (fun _ => wtVar mem).
+
+    Definition Uvar {tus tvs} {ts t} (mem : member (ts,t) tus)
+    : logicA m
+             (fun tus tvs => hlist (wtexpr Esymbol tus tvs) ts)
+             (fun tus tvs => wtexpr Esymbol tus tvs t)
+             tus tus tvs :=
+      pureA (fun hl => wtUVar mem hl).
+*)
